updating

coq/NonSpeculativeConcrete.v
@@ -3,8 +3,11 @@ From Coq Require Import List.
 Import ListNotations.
 
 From SE Require Import BitVectors.
+From SE Require Import CFG.
 From SE Require Import Concrete.
 From SE Require Import DynamicValue.
+From SE Require Import LLVMAst.
+From SE Require Import Relation.
 
 Inductive store_has_no_poison : dv_store -> Prop :=
   | Store_Has_No_Poison : forall ls,
@@ -47,3 +50,20 @@ Inductive ns_step : state -> state -> Prop :=
   | NS_Step : forall s1 s2,
       step s1 s2 -> has_no_poison s2 -> ns_step s1 s2
 .
+
+Definition multi_ns_step := multi ns_step.
+
+Definition is_safe_program_with_ns_step (mdl : llvm_module) (fid : function_id) :=
+  exists init_s,
+    (init_state mdl fid) = Some init_s /\ (forall s, multi_ns_step init_s s -> ~ error_state s)
+.
+
+Lemma ns_step_soundness : forall s1 s2,
+  ns_step s1 s2 -> step s1 s2.
+Proof.
+Admitted.
+
+Lemma multi_ns_step_soundness : forall s1 s2,
+  multi_ns_step s1 s2 -> multi_step s1 s2.
+Proof.
+Admitted.
